theories/prob_eff_lang/probblaze/examples/DH_KE/advantage_comp.v
@@ -3,6 +3,7 @@ From iris.algebra Require Import excl.
 From iris.algebra.lib Require Import dfrac_agree.
 From clutch.prob_eff_lang.probblaze Require Import sec_channel_def p_composition sem_def sem_types sem_judgement sem_row syntax semantics proofmode valgroup adequacy.
 From clutch.prob_eff_lang.probblaze Require Import new_composition xor new_composition_defs def_dhke.
+From clutch.prob_eff_lang.probblaze.examples.DH_KE Require Import advantage_dhke_lazy.
 
 Section adv_comp.
   Context {vg : val_group} {cg : clutch_group_struct} {vgg : @val_group_generator vg}.
@@ -11,19 +12,16 @@ Section adv_comp.
   Context `{Hpre :probblazeRGpreS Σ}.
   Let Key := S (S n'').
   Let Support := S (S n'').
-  Variable xor_struct : XOR (Key := Key) (Support := Support).
+  Context {xor_struct : XOR (Key := Key) (Support := Support)}.
   Context `{X : ∀ `{!probblazeRGS Σ}, XOR_spec (Key := Key) (Support := Support) (H := xor_struct)}.
 
 
   Theorem adv_composition A :
      (∀ `{!probblazeRGS Σ},⊢ sem_val_typed A A (τ → 𝔹)%T) →
-    advantage A
-      (REAL_CHAN_DHKE xor_struct)
-      SIMSIMFCHAN #true
-    <= advantage A 
-                 (REAL_CHAN_DH_REAL xor_struct)
-                 (REAL_CHAN_DH_RAND xor_struct) #true.
-  Proof using G Hpre Key Support X cg inG0 inG1 inG2 vg vgg xor_struct Σ. 
+     advantage A REAL_CHAN_DHKE SIMSIMFCHAN #true
+    <=
+      advantage A REAL_CHAN_DH_REAL REAL_CHAN_DH_RAND #true.
+  Proof using G Hpre Key Support X cg inG0 inG1 inG2 vg vgg xor_struct Σ.
     intros Hadv.
     eapply (advantage_triangle _ _ _ _ _ 0); last (rewrite Rplus_0_l; apply Rle_refl).
     - right. eapply sem_val_typed_advantage; first apply Hadv.
@@ -57,22 +55,53 @@ Section adv_comp.
       + intros H. by apply SIMFCHAN_DHSIM_FKE_CHAN4. 
   Qed. 
 
+
+  Lemma REAL_DHKE_DH_RED_RAND_adv (A : val) (b : bool) :
+    (∀ `{!probblazeRGS Σ}, ⊢ sem_val_typed A A (τ → 𝔹)%T) →
+    nonneg $ advantage A REAL_CHAN_DH_RED_RAND REAL_CHAN_DH_RAND #b = 0.
+  Proof using All.
+    intros Aty.
+    eapply sem_typed_advantage.
+    1: apply Aty.
+    split ; intros.
+    - by eapply REAL_DHKE_DH_RED_RAND'.
+    - simpl. by eapply REAL_DHKE_DH_RED_RAND.
+  Qed.
+
+  Lemma REAL_DHKE_DH_RED_REAL_adv (A : val) (b : bool) :
+    (∀ `{!probblazeRGS Σ}, ⊢ sem_val_typed A A (τ → 𝔹)%T) →
+    nonneg $ advantage A REAL_CHAN_DH_RED_REAL REAL_CHAN_DH_REAL #b = 0.
+  Proof using All.
+    intros Aty.
+    eapply sem_typed_advantage.
+    1: apply Aty.
+    split ; intros.
+    - by eapply REAL_DHKE_DH_RED_REAL'.
+    - simpl. by eapply REAL_DHKE_DH_RED_REAL.
+  Qed.
+
   Theorem adv_composition_real A :
     (∀ `{!probblazeRGS Σ},⊢ sem_val_typed A A (τ → 𝔹)%T) →
-    advantage A (REAL_CHAN_DHKE xor_struct) SIMSIMFCHAN #true <=
-      advantage (λ: "v", A (((λ: "DH", λ: "f", (((λ: "f", F_AUTH (C_lazy "DH" "f")))%V ||ᵣ F_OAUTH) "f") "v")))%V DH_real DH_rand #true.
+    advantage A REAL_CHAN_DHKE SIMSIMFCHAN #true <=
+      advantage (λ: "v", A ((REAL_CHAN_DH_RED "v")))%V DH_real DH_rand #true.
   Proof using G Hpre Key Support X cg inG0 inG1 inG2 vg vgg xor_struct Σ. 
-    intros.
+    intros Aty.
     etrans. 
     - apply adv_composition; eauto.
-    -                           (* A lemma relating REAL_CHAN_DH_REAL and REAL_CHAN_DH_RAND is needed, where they first take DDH as arguments *)
-(* eapply advantage_reduction. 
-         intros ?. eexists _,_.
-         split; try done.
-         split.
-         + admit.
-         + admit.
-     Admitted.  *)
-  Admitted. 
+    - eapply (advantage_triangle _ _ _ _ _ 0 _); last try lra.
+      3: rewrite Rplus_0_l ; reflexivity.
+      2: eapply (advantage_triangle _ _ _ _ _ _ 0); last try lra.
+      4: rewrite Rplus_0_r ; reflexivity.
+      { right. rewrite advantage_sym.
+        apply REAL_DHKE_DH_RED_REAL_adv. done. }
+      2: { right. apply REAL_DHKE_DH_RED_RAND_adv. done. }
+      apply (advantage_reduction A REAL_CHAN_DH_RED DH_real DH_rand true).
+      intros. eexists _,_. split ; [|split].
+      1: apply Aty.
+      2:{ split.
+          - by unshelve eapply DH_real_self.
+          - by unshelve eapply DH_rand_self. }
+      apply REAL_CHAN_DH_RED_sem_typed.
+  Qed.
 
 Section adv_comp.
